compiler/core/Translation/ErgoNNRCtoErgoImp.v
@@ -19,6 +19,7 @@ Require Import List.
 
 Require Import Qcert.JavaScriptAst.JavaScriptAstRuntime.
 Require Import Qcert.Driver.CompDriver.
+Require Import Qcert.Driver.CompCorrectness.
 Require Import ErgoSpec.Version.
 Require Import ErgoSpec.Utils.Misc.
 Require Import ErgoSpec.Common.Result.
@@ -70,5 +71,184 @@ Section ErgoNNRCtoErgoImp.
   End Translation.
 
   Section Correctness.
+    Definition same_result (r1 r2:eresult qcert_data) :=
+      match r1, r2 with
+      (* Either both successful with the same data *)
+      | Success _ _ d1, Success _ _ d2 => d1 = d2
+      (* Or both fail with any error *)
+      | Failure _ _ e1, Failure _ _ e2 => True
+      (* Otherwise the result is different *)
+      | _, _ => False
+      end.
+
+    Notation "r1 ≡ r2" := (same_result r1 r2) (at level 90).
+
+    Lemma ergo_function_lookup_correct s l:
+      ergo_imp_declaration_lookup_function s (ergo_nnrc_declarations_to_imp l)
+      = lift (ergo_nnrc_function_to_imp nil) (ergo_nnrc_declaration_lookup_function s l).
+    Proof.
+      induction l; intros; try reflexivity; simpl.
+      destruct a; simpl; try assumption.
+      destruct (string_dec s0 s); try assumption; subst.
+      reflexivity.
+    Qed.
+
+    Lemma ergo_function_table_lookup_correct s l:
+      ergo_imp_declaration_lookup_table s (ergo_nnrc_declarations_to_imp l)
+      = lift (ergo_nnrc_function_table_to_imp nil) (ergo_nnrc_declaration_lookup_table s l).
+    Proof.
+      induction l; intros; try reflexivity; simpl.
+      destruct a; simpl; try assumption.
+      destruct (string_dec s0 s); try assumption; subst.
+      reflexivity.
+    Qed.
+      
+    Lemma ergo_function_in_function_table_lookup_correct s l :
+      lift
+        (ergo_nnrc_function_to_imp nil)
+        (lookup string_dec l s) =
+      (lookup string_dec
+              (map (fun xy : string * ergo_nnrc_lambda => (fst xy, ergo_nnrc_function_to_imp nil (snd xy)))
+                   l) s).
+    Proof.
+      induction l; intros; try reflexivity; simpl.
+      destruct a; simpl in *.
+      destruct (string_dec s s0); try reflexivity.
+      rewrite IHl.
+      reflexivity.
+    Qed.
+
+    Lemma ergo_nnrc_lambda_to_imp_correct (f:ergo_nnrc_lambda) :
+      forall params: list (string * qcert_data),
+        ergo_nnrc_lambda_eval f params ≡ ergo_imp_lambda_eval (ergo_nnrc_function_to_imp nil f) params.
+    Proof.
+      intros.
+      unfold ergo_nnrc_lambda_eval.
+      unfold ergo_imp_lambda_eval.
+      unfold CompEval.eval_nnrc.
+      unfold CompEval.h.
+      unfold ergo_nnrc_function_to_imp.
+      unfold QcertCodeGen.nnrc_expr_to_imp_ejson_function.
+      rewrite (@eval_nnrc_to_imp_correct _ _ _ _ _ bm).
+      unfold CompEval.h.
+      unfold nnrc_expr_to_imp_ejson_function.
+      assert (
+          (@lift (@EJson.ejson QcertEJson.enhanced_foreign_ejson)
+          (@data (@foreign_runtime_data QcertData.enhanced_foreign_runtime))
+          (@DataToEJson.ejson_to_data QcertData.enhanced_foreign_runtime QcertEJson.enhanced_foreign_ejson
+             QcertDataToEJson.enhanced_foreign_to_ejson)
+          (@ImpEJsonEval.imp_ejson_function_eval QcertEJson.enhanced_foreign_ejson
+             (@ForeignDataToEJson.foreign_to_ejson_runtime QcertData.enhanced_foreign_runtime
+                QcertEJson.enhanced_foreign_ejson QcertDataToEJson.enhanced_foreign_to_ejson)
+             (@brand_relation_brands (@brand_model_relation QcertType.enhanced_foreign_type bm))
+             (@ImpDatatoImpEJson.imp_data_function_to_imp_ejson QcertData.enhanced_foreign_runtime
+                QcertEJson.enhanced_foreign_ejson QcertDataToEJson.enhanced_foreign_to_ejson
+                (@ForeignDataToEJson.foreign_to_ejson_runtime QcertData.enhanced_foreign_runtime
+                   QcertEJson.enhanced_foreign_ejson QcertDataToEJson.enhanced_foreign_to_ejson)
+                QcertDataToEJson.enhanced_foreign_to_ejson_runtime
+                (@CompEval.h QcertType.enhanced_foreign_type bm)
+                (@NNRSimptoImpData.nnrs_imp_to_imp_data_function QcertData.enhanced_foreign_runtime
+                   (@nnrs_to_nnrs_imp QcertData.enhanced_foreign_runtime
+                      (@nnrc_to_nnrs QcertData.enhanced_foreign_runtime (@nil string) (@lambdan_body bm f)))))
+             (@EJson.ejobject QcertEJson.enhanced_foreign_ejson
+                (@rec_sort string ODT_string (@EJson.ejson QcertEJson.enhanced_foreign_ejson)
+                   (@map (prod string (@data (@foreign_runtime_data QcertData.enhanced_foreign_runtime)))
+                      (prod string (@EJson.ejson QcertEJson.enhanced_foreign_ejson))
+                      (fun xy : prod string (@data (@foreign_runtime_data QcertData.enhanced_foreign_runtime)) =>
+                       @pair string (@EJson.ejson QcertEJson.enhanced_foreign_ejson)
+                         (key_encode
+                            (@fst string (@data (@foreign_runtime_data QcertData.enhanced_foreign_runtime)) xy))
+                         (@DataToEJson.data_to_ejson QcertData.enhanced_foreign_runtime
+                            QcertEJson.enhanced_foreign_ejson QcertDataToEJson.enhanced_foreign_to_ejson
+                            (@snd string (@data (@foreign_runtime_data QcertData.enhanced_foreign_runtime)) xy)))
+                      params)))))
+          = (@lift (@EJson.ejson QcertEJson.enhanced_foreign_ejson)
+          (@data (@foreign_runtime_data QcertData.enhanced_foreign_runtime))
+          (@DataToEJson.ejson_to_data QcertData.enhanced_foreign_runtime QcertEJson.enhanced_foreign_ejson
+             QcertDataToEJson.enhanced_foreign_to_ejson)
+          (@ImpEJsonEval.imp_ejson_function_eval QcertEJson.enhanced_foreign_ejson
+             QcertEJson.enhanced_foreign_ejson_runtime
+             (@brand_relation_brands (@brand_model_relation QcertType.enhanced_foreign_type bm))
+             (@ImpDatatoImpEJson.imp_data_function_to_imp_ejson QcertData.enhanced_foreign_runtime
+                QcertEJson.enhanced_foreign_ejson QcertDataToEJson.enhanced_foreign_to_ejson
+                (@ForeignDataToEJson.foreign_to_ejson_runtime QcertData.enhanced_foreign_runtime
+                   QcertEJson.enhanced_foreign_ejson QcertDataToEJson.enhanced_foreign_to_ejson)
+                QcertDataToEJson.enhanced_foreign_to_ejson_runtime
+                (@CompEval.h QcertType.enhanced_foreign_type bm)
+                (@NNRSimptoImpData.nnrs_imp_to_imp_data_function QcertData.enhanced_foreign_runtime
+                   (@nnrs_to_nnrs_imp QcertData.enhanced_foreign_runtime
+                      (@nnrc_to_nnrs QcertData.enhanced_foreign_runtime (@nil string) (@lambdan_body bm f)))))
+             (@EJson.ejobject QcertEJson.enhanced_foreign_ejson
+                (@rec_sort string ODT_string (@EJson.ejson QcertEJson.enhanced_foreign_ejson)
+                   (@map (prod string (@data (@foreign_runtime_data QcertData.enhanced_foreign_runtime)))
+                      (prod string (@EJson.ejson QcertEJson.enhanced_foreign_ejson))
+                      (fun xy : prod string (@data (@foreign_runtime_data QcertData.enhanced_foreign_runtime)) =>
+                       @pair string (@EJson.ejson QcertEJson.enhanced_foreign_ejson)
+                         (key_encode
+                            (@fst string (@data (@foreign_runtime_data QcertData.enhanced_foreign_runtime)) xy))
+                         (@DataToEJson.data_to_ejson QcertData.enhanced_foreign_runtime
+                            QcertEJson.enhanced_foreign_ejson QcertDataToEJson.enhanced_foreign_to_ejson
+                            (@snd string (@data (@foreign_runtime_data QcertData.enhanced_foreign_runtime)) xy)))
+                      params)))))
+        ) by reflexivity.
+      rewrite H; clear H.
+      destruct (@lift (@EJson.ejson QcertEJson.enhanced_foreign_ejson)
+          (@data (@foreign_runtime_data QcertData.enhanced_foreign_runtime))
+          (@DataToEJson.ejson_to_data QcertData.enhanced_foreign_runtime QcertEJson.enhanced_foreign_ejson
+             QcertDataToEJson.enhanced_foreign_to_ejson)
+          (@ImpEJsonEval.imp_ejson_function_eval QcertEJson.enhanced_foreign_ejson
+             QcertEJson.enhanced_foreign_ejson_runtime
+             (@brand_relation_brands (@brand_model_relation QcertType.enhanced_foreign_type bm))
+             (@ImpDatatoImpEJson.imp_data_function_to_imp_ejson QcertData.enhanced_foreign_runtime
+                QcertEJson.enhanced_foreign_ejson QcertDataToEJson.enhanced_foreign_to_ejson
+                (@ForeignDataToEJson.foreign_to_ejson_runtime QcertData.enhanced_foreign_runtime
+                   QcertEJson.enhanced_foreign_ejson QcertDataToEJson.enhanced_foreign_to_ejson)
+                QcertDataToEJson.enhanced_foreign_to_ejson_runtime
+                (@CompEval.h QcertType.enhanced_foreign_type bm)
+                (@NNRSimptoImpData.nnrs_imp_to_imp_data_function QcertData.enhanced_foreign_runtime
+                   (@nnrs_to_nnrs_imp QcertData.enhanced_foreign_runtime
+                      (@nnrc_to_nnrs QcertData.enhanced_foreign_runtime (@nil string) (@lambdan_body bm f)))))
+             (@EJson.ejobject QcertEJson.enhanced_foreign_ejson
+                (@rec_sort string ODT_string (@EJson.ejson QcertEJson.enhanced_foreign_ejson)
+                   (@map (prod string (@data (@foreign_runtime_data QcertData.enhanced_foreign_runtime)))
+                      (prod string (@EJson.ejson QcertEJson.enhanced_foreign_ejson))
+                      (fun xy : prod string (@data (@foreign_runtime_data QcertData.enhanced_foreign_runtime)) =>
+                       @pair string (@EJson.ejson QcertEJson.enhanced_foreign_ejson)
+                         (key_encode
+                            (@fst string (@data (@foreign_runtime_data QcertData.enhanced_foreign_runtime)) xy))
+                         (@DataToEJson.data_to_ejson QcertData.enhanced_foreign_runtime
+                            QcertEJson.enhanced_foreign_ejson QcertDataToEJson.enhanced_foreign_to_ejson
+                            (@snd string (@data (@foreign_runtime_data QcertData.enhanced_foreign_runtime)) xy)))
+                      params))))); simpl; auto.
+    Qed.
+
+    (** Main theorem of correctness for ErgoNNRC to ErgoImp translation.
+
+        It states that invoking a contract on ErgoNNRC yields the same
+        result (same successful evaluation or same error) as invoking
+        a contract on that contract translated to ErgoImp *)
+
+    Theorem ergo_nnrc_to_imp_correct (m : ergo_nnrc_module) :
+      forall callname : (option string * string),
+      forall params: list (string * qcert_data),
+        ergo_nnrc_invoke m callname params ≡ ergo_imp_invoke (ergo_nnrc_module_to_imp m) callname params.
+    Proof.
+      intros.
+      destruct callname.
+      destruct o; simpl.
+      (* Proof for contract invoke *)
+      - rewrite ergo_function_table_lookup_correct; simpl.
+        Opaque ergo_imp_declaration_lookup_function.
+        destruct (ergo_nnrc_declaration_lookup_table s (modulen_declarations m)); try reflexivity; simpl.
+        unfold ergo_nnrc_function_table_eval.
+        rewrite <- ergo_function_in_function_table_lookup_correct.
+        destruct (lookup string_dec (function_tablen_funs e) s); try reflexivity; simpl.
+        apply ergo_nnrc_lambda_to_imp_correct.
+      (* Proof for function invoke *)
+      - rewrite ergo_function_lookup_correct; simpl.
+        destruct (ergo_nnrc_declaration_lookup_function s (modulen_declarations m)); try reflexivity; simpl.
+        apply ergo_nnrc_lambda_to_imp_correct.
+    Qed.
+
   End Correctness.
 End ErgoNNRCtoErgoImp.
